examples/Common/CASMemSpec.v
@@ -1,0 +1,109 @@
+Require Import FMapPositive.
+Require Import Relation_Operators Operators_Properties.
+Require Import Coq.PArith.PArith.
+Require Import Coq.Program.Equality.
+Require Import PeanoNat.
+
+Require Import coqrel.LogicalRelations.
+Require Import models.EffectSignatures.
+Require Import examples.Common.Heap.
+Require Import examples.Common.AtomicLTS.
+Require Import LinCCAL.
+Require Import LTS.
+Require Import TPSimulationSet.
+
+
+(** A heap of CAS registers: the address-indexed counterpart of
+    [CASRegSpec.ECASReg].  It mirrors [MemSpec.WriteRacyMem], except that
+    cells are only ever updated with [ccas], so there is no write race and
+    no racy error.  [cmalloc] takes the initial value of the fresh cell. *)
+Module CASMemSpec.
+  Import LTSSpec.
+  Import LinCCALBase.
+  Import AtomicLTS.
+  Import TPSimulationSet.TPSimulation.
+
+  Variant ECASMem_op {A} :=
+  | cmalloc (v : A)
+  | cget (addr : Addr)
+  | ccas (addr : Addr) (v w : A).
+  Arguments ECASMem_op : clear implicits.
+
+  Definition ECASMem_ar {A} (m : ECASMem_op A) : Type :=
+    match m with
+    | cmalloc _ => Addr
+    | cget _ => A
+    | ccas _ _ _ => bool
+    end.
+
+  Canonical Structure ECASMem A :=
+  {|
+    Sig.op := ECASMem_op A;
+    Sig.ar := ECASMem_ar
+  |}.
+
+  Module CASMem.
+    Definition CASMemState {A} := @Heap A.
+
+    Variant StepCASMem {A} :
+      @ThreadEvent (ECASMem A) -> CASMemState -> CASMemState -> Prop :=
+    (* alloc steps *)
+    | step_alloc_inv t h v e :
+      e = {| te_tid := t; te_ev := InvEv (cmalloc v) |} ->
+      StepCASMem e h h
+    | step_alloc_res t h l v e :
+      e = {| te_tid := t; te_ev := ResEv (cmalloc v) l |} ->
+      h l = None ->
+      StepCASMem e h (heap_update l v h)
+    (* read steps *)
+    | step_get_inv t l h e :
+      e = {| te_tid := t; te_ev := InvEv (cget l) |} ->
+      h l <> None ->
+      StepCASMem e h h
+    | step_get_res t l h v e :
+      e = {| te_tid := t; te_ev := ResEv (cget l) v |} ->
+      h l = Some v ->
+      StepCASMem e h h
+    (* cas steps *)
+    | step_cas_inv t l v w h e :
+      e = {| te_tid := t; te_ev := InvEv (ccas l v w) |} ->
+      h l <> None ->
+      StepCASMem e h h
+    | step_cas_res_succ t l v w h e :
+      e = {| te_tid := t; te_ev := ResEv (ccas l v w) true |} ->
+      h l = Some v ->
+      StepCASMem e h (heap_update l w h)
+    | step_cas_res_fail t l u v w h e :
+      e = {| te_tid := t; te_ev := ResEv (ccas l v w) false |} ->
+      h l = Some u ->
+      u <> v ->
+      StepCASMem e h h.
+
+    Variant ErrorCASMem {A} :
+      @ThreadEvent (ECASMem A) -> (@AState (ECASMem A) (@CASMemState A)) -> Prop :=
+    | error_get_undefined t h l e :
+      e = {| te_tid := t; te_ev := InvEv (cget l) |} ->
+      h l = None ->
+      ErrorCASMem e (Idle h)
+    | error_cas_undefined t h l v w e :
+      e = {| te_tid := t; te_ev := InvEv (ccas l v w) |} ->
+      h l = None ->
+      ErrorCASMem e (Idle h).
+
+    Definition VCASMem {A} : @LTS (ECASMem A) := VAE StepCASMem ErrorCASMem.
+  End CASMem.
+
+  Module CASMemLayer.
+    Section Impl.
+      Context {A : Type}.
+
+      Definition L : layer_interface :=
+      {|
+        li_sig := ECASMem A;
+        li_lts := CASMem.VCASMem;
+        li_init := Idle empty_heap;
+      |}.
+    End Impl.
+  End CASMemLayer.
+
+End CASMemSpec.
